test-suite/rec.v
@@ -16,6 +16,106 @@ Module RecRel.
 
 End RecRel.
 
+Definition gt_bound n : relation nat :=
+  fun x y => x > y /\ x < n.
+
+Definition minus_12 n := 
+  if le_lt_dec n 100 then n - 12 else n.
+
+Instance gt_bound_wf n : WellFounded (gt_bound n).
+Proof. red. red. intros.
+  Admitted.
+
+
+Equations f91 n : { m : nat | n < m - 11 } :=
+f91 n by rec n (gt_bound 100) :=
+f91 n with le_lt_dec n 100 := {
+  | left H := exist _ (proj1_sig (f91 (proj1_sig (f91 (n + 11))))) _ ;
+  | right H := exist _ (n - 10) _ }.
+
+Admit Obligations.
+
+Next Obligation. apply f91. red.
+  unfold minus_12. destruct (le_lt_dec n 100).
+  destruct le_lt_dec.
+  simpl. admit.
+
+
+Section Nested.
+
+  Equations f (n : nat) : { x : nat | x <= n } :=
+  f n by rec n lt :=
+  f 0 := exist _ 0 _ ;
+  f (S n) := exist _ (proj1_sig (f (proj1_sig (f n)))) _.
+
+  Next Obligation. destruct_call f_comp_proj. simpl. exists x. auto. Defined.
+  Next Obligation. do 2 destruct_call f_comp_proj. simpl in *. eauto with arith. Defined.
+
+  Next Obligation. do 2 destruct_call f. simpl in *. eauto with arith. Defined.
+
+  Next Obligation. admit. Defined. 
+
+  Next Obligation. 
+    rec_wf_rel n IH lt.
+    destruct x. constructor. simp f.
+    constructor. intros. subst recres. auto.
+    auto. apply IH. destruct f. auto with arith.
+  Defined.
+
+About f_elim.
+
+End Nested.
+Require Import Coq.Lists.SetoidList.
+Require Import Coq.Sorting.Sorting.
+Require Import Coq.Sorting.Permutation.
+Require Import Coq.Sorting.PermutSetoid.
+
+Print Instances Morphisms.Proper.
+
+Instance filter_ext {A} : Morphisms.Proper (pointwise_relation A eq ==> eq ==> eq) (@filter A).
+Proof.
+  reduce. subst. induction y0; simpl; auto. generalize (H a). case_eq (x a). intros _ <-; congruence.
+  intros _ <-; congruence.
+Qed.
+
+Lemma Permutation_filter {A} (l : list A)
+  (p : A -> bool) : Permutation l (filter p l ++ filter (compose negb p) l).
+Proof with simpl; intros.
+  induction l; unfold compose; simpl; auto.
+  case_eq (p a); simpl; intros;
+  auto using Permutation_cons_app. 
+Qed.
+
+Inductive xor (A B : Prop) : Prop :=
+| xor_left : A -> not B -> xor A B
+| xor_right : B -> not A -> xor A B.
+
+Require Import Bool.
+Coercion Is_true : bool >-> Sortclass.
+
+Lemma xor_reflect (x y : bool) : reflect (xor x y) (xorb x y).
+Proof.
+  destruct x; destruct y; simpl; auto;
+  constructor; try (intro H; elim H); firstorder.
+Qed.
+
+Lemma Permutation_filter2 {A} (l : list A)
+  (p q : A -> bool) : 
+  (forall x, xorb (p x) (q x)) ->
+  Permutation l (filter p l ++ filter q l).
+Proof with simpl; intros. intros.
+  induction l; unfold compose; simpl; auto.
+  generalize (H a).
+  case_eq (p a); simpl; intros.
+  apply Permutation_cons. revert H1. 
+  case_eq (q a); intros qa; intros; try discriminate. elim H1.
+  apply IHl.
+
+  revert H1. 
+  case_eq (q a); intros qa; intros; try discriminate.
+  auto using Permutation_cons_app. elim H1.
+Qed.
+
 Module RecMeasure.
   
   Equations id (n : nat) : nat :=
@@ -52,22 +152,38 @@ Module RecMeasure.
     Hint Unfold lt gt : Below.
     Hint Resolve le_lt_n_Sm : Below.
 
-    Context {A : Type} (leb : A -> A -> bool).
+    Context {A : Type} (leb : A -> A -> bool) (ltb : A -> A -> bool).
 
     Equations qs (l : list A) : list A :=
     qs l by rec l (MR lt (@length A)) :=
     qs nil := nil ;
     qs (cons a l) := 
-      let lower := filter (fun x => leb x a) l in
+      let lower := filter (fun x => ltb x a) l in
       let upper := filter (fun x => leb a x) l in
         qs lower ++ a :: qs upper.
 
-    Context (R : relation A).
-    Context (refl : forall x y, reflect (R x y) (leb x y)).
+    Context (le : relation A).
+    Context (refl_le : forall x y, reflect (le x y) (leb x y)).
 
-    Context (leb_complete : forall x y, leb x y = true <-> (x = y \/ leb y x = false)).
-    Context (leb_complete2 : forall x y, leb x y = false -> leb y x = true).
-    
+    Context (lt : relation A).
+    Context (refl_lt : forall x y, reflect (lt x y) (ltb x y)).
+
+    Context (leb_complete : forall x y, leb x y <-> (x = y \/ leb y x = false)).
+    Context (leb_complete2 : forall x y, leb x y = false -> leb y x).
+
+    Context (ltb_leb : forall x y, ltb x y -> leb x y).
+    Context (nltb_leb : forall x y, ltb x y = false -> leb y x).
+(*     Context (ltb_leb' : forall x y, ltb x y = false -> (x = y \/ leb y x = true)). *)
+    Context (ltb_leb' : forall x y, leb x y = false <-> ltb y x).
+    Context (ltb_leb'' : forall x y, ltb x y <-> ~ leb y x).
+
+    About filter_In.
+    Lemma filter_In' :
+      ∀ (A : Type) (f : A → bool) (x : A) (l : list A),
+      In x (filter f l) ↔ In x l ∧ f x.
+    Proof.
+      intros. rewrite filter_In. intuition. apply Is_true_eq_true; auto.
+    Qed.
 
     Lemma qs_same (l : list A) : forall a, In a l <-> In a (qs l).
     Proof. intros.
@@ -78,19 +194,113 @@ Module RecMeasure.
       intros.
       simpl. split; intros.
       destruct H1. subst. auto with datatypes.
-      case_eq (leb a a0); intros eq.
+      case_eq (leb a a0); intros eq. 
+      apply Is_true_eq_left in eq.
       rewrite leb_complete in eq.
       destruct eq. subst. rewrite in_app_iff. right; left; auto.
       
-      rewrite filter_In in H.
-      rewrite in_app_iff. left. apply H. auto.
+      rewrite filter_In' in H.
+      rewrite in_app_iff. left. apply H. rewrite ltb_leb' in H2. auto.
       
-      rewrite filter_In in H0.
+      rewrite filter_In' in H0. 
       rewrite in_app_iff. right. right. apply H0. auto.
       
-      rewrite in_app_iff in H1. destruct H1. rewrite <- H, filter_In in H1. tauto.
-      apply in_inv in H1. destruct H1; auto. right. rewrite <- H0 in H1. rewrite filter_In in H1. tauto.
+      rewrite in_app_iff in H1. destruct H1. rewrite <- H, filter_In' in H1. tauto.
+      apply in_inv in H1. destruct H1; auto. right. rewrite <- H0 in H1. rewrite filter_In' in H1. tauto.
     Qed.
+
+    Lemma sort_le_app :
+      forall l1 l2, sort le l1 -> sort le l2 ->
+        (forall x y, In x l1 -> In y l2 -> le x y) ->
+        sort le (l1 ++ l2).
+    Proof.
+      induction l1; simpl in *; intuition.
+      inversion_clear H.
+      constructor; auto.
+      apply InfA_app; auto.
+      destruct l2; auto.
+      constructor ; auto.
+      auto with datatypes.
+    Qed.
+  
+    Lemma hd_rel_all a l : (forall x, In x l -> le a x) -> HdRel le a l.
+    Proof. intros H. induction l; auto.
+      constructor. apply H. auto with datatypes.
+    Qed.
+
+    Lemma hdrel_filter a l : HdRel le a (qs (filter (λ x : A, leb a x) l)).
+    Proof. apply hd_rel_all. 
+      intros. rewrite <- qs_same in H. rewrite filter_In in H. destruct H.
+      pose (refl_le a x). now depelim r.
+    Qed.
+   
+    Context `(le_trans : Transitive A le).
+
+    Lemma qs_sort (l : list A) : sort le (qs l).
+    Proof. intros.
+      pattern_call (qs l).
+      let p := constr:(fun_elim (f:=@qs)) in apply p.
+      constructor.
+
+      intros.
+      apply sort_le_app; auto.
+      constructor. auto. apply hdrel_filter.
+      intros. simpl in H2.
+      rewrite <- qs_same, filter_In' in H1, H2.
+      intuition auto with arith. subst. pose (r:=refl_le x y); apply ltb_leb in H4; now depelim r.
+      apply ltb_leb in H4.
+      pose (r:=refl_le x a); pose (r':=refl_le a y); depelim r; depelim r'; reverse; simplify_dep_elim; auto. 
+      transitivity a; auto. elim H5.  elim H4. elim H4.
+    Qed.
+    Require Import EquivDec.
+    Require Import Permutation.
+    Existing Instance Permutation_app'_Proper.
+
+(*     Lemma leb_negb a : (fun x => leb a x) === compose negb (fun x => leb x a). *)
+(*     Proof. *)
+(*       unfold negb, compose. intros x.  *)
+(*       case_eq (leb a x); intros H. *)
+(*       apply leb_complete in H. destruct H. subst. admit. *)
+(*       now rewrite H. *)
+(*       apply leb_complete2 in H. *)
+(*       now rewrite H. *)
+(*     Qed. *)
+(*     Typeclasses eauto :=. *)
+
+(*     Lemma leb_negb' a : (fun x => leb x a) === compose negb (fun x => leb a x). *)
+(*     Proof. *)
+(*       unfold negb, compose. intros x.  *)
+(*       case_eq (leb x a); intros H. *)
+(*       apply leb_complete in H. destruct H. subst. admit. *)
+(*       now rewrite H. *)
+(*       apply leb_complete2 in H. *)
+(*       now rewrite H. *)
+(*     Qed. *)
+(*     Typeclasses eauto :=. *)
+
+    Lemma qs_perm l : Permutation l (qs l).
+    Proof.
+      pattern_call (qs l).
+      let p := constr:(fun_elim (f:=@qs)) in apply p.
+      constructor.
+      intros. 
+      rewrite <- H0, <- H.
+      apply Permutation_cons_app.
+      rewrite Permutation_app_comm.
+      apply Permutation_filter2.
+      intros. case_eq (leb a x). simpl.
+      intros.
+      case_eq (ltb x a). intros. 
+      apply Is_true_eq_left in H2.
+      apply Is_true_eq_left in H1.
+      apply ltb_leb'' in H2. contradiction.
+      constructor.
+      simpl.
+      intros.
+      rewrite ltb_leb' in H1. case_eq (ltb x a). constructor.
+      intros. rewrite H2 in H1. elim H1.
+    Qed.
+  
   End QuickSort.
 
 End RecMeasure.
@@ -104,6 +314,8 @@ Section Nested.
 
   Next Obligation. destruct_call f_comp_proj. simpl. exists x. auto. Defined.
   Next Obligation. do 2 destruct_call f_comp_proj. simpl in *. eauto with arith. Defined.
+    Set Printing All.
+  Print f_obligation_2.
 
   Next Obligation. do 2 destruct_call f. simpl in *. eauto with arith. Defined.
 
@@ -116,5 +328,4 @@ Section Nested.
     auto. apply IH. destruct f. auto with arith.
   Defined.
 
-
-  About f_elim.
+End Nested.
